# 第二章　ラムゼイモデル：最適化行動の導入



## 2.4　ラムゼイモデル


$$
U_t^{(j)}= \sum_{i=0}^{\infty}\beta^{i}u(C_{t+i})
$$

$$
K_{t+1}^{(j)}-K_t^{(j)}=r_tK_t^{(j)}+w_t^{(j)}-C_t^{(j)}-\delta K_t^{(j)}
$$

$$
\max_{c} U_t^{(j)}= \sum_{i=0}^{\infty}\beta^{i}u(C_{t+i})\\
s.t. ~K_{t+1}^{(j)}-K_t^{(j)}=r_tK_t^{(j)}+w_t^{(j)}-C_t^{(j)}-\delta K_t^{(j)}
$$

$$
\begin{align}
\mathcal{L}&=\sum_{i=0}^{\infty}\beta^{i}u(C_{t+i})+\sum_{i=t}^{\infty}\lambda_i'(r_tK_t+w_t-C_t+(1-\delta) K_t-K_{t+1})\\
&=\sum_{i=t}^{\infty}\beta^{i-t}u(C_{i})+\sum_{i=t}^{\infty}\lambda_i'(r_tK_t+w_t-C_t+(1-\delta) K_t-K_{t+1})\\
&=\sum_{i=t}^{\infty}\beta^{i-t} \left[u(C_{i})+\lambda_i(r_tK_t+w_t-C_t+(1-\delta) K_t-K_{t+1}) \right]\\
\end{align}
$$

$$
\begin{align}
\frac{\part{\mathcal{L}}}{C_{t}}=0 ~&\Rightarrow~ u'(C_t)=\lambda_t \\
\frac{\part{\mathcal{L}}}{C_{t+1}}=0 ~&\Rightarrow~ u'(C_{t+1})=\lambda_{t+1} \\
\frac{\part{\mathcal{L}}}{K_{t+1}}=0 ~&\Rightarrow~ -\lambda_t+\lambda_{t+1}\beta(r_{t+1}+1-\delta)=0\\
\end{align}
$$


$$
\begin{align}
\frac{1}{C_t}=\lambda_t\\
\frac{1}{C_{t+1}}=\lambda_{t+1}\\
\end{align}
$$

$$
\frac{C_{t+1}}{C_t}=\beta(r_{t+1}+1-\delta)
$$


$$
Y_t^{k}=A_t^{k}(K_t^{k})^{\alpha}(L_t^{k})^{1-\alpha}
$$

$$
\max_{K_t,L_t} \Pi = Y_t-r_tK_t-w_tL_t\\
s.t.~Y_t=A_tK_t^\alpha L_t^{1-\alpha}
$$

$$
\max_{K_t,L_t} \Pi = A_tK_t^\alpha L_t^{1-\alpha}-r_tK_t-w_tL_t
$$


$$
\begin{align}
\frac{\part{\Pi}}{\part{K_{t}}}=0 ~&\Rightarrow~ \alpha A_tK_t^{\alpha-1}L_t^{1-\alpha}=r_t\\
\frac{\part{\Pi}}{\part{L_{t}}}=0 ~&\Rightarrow~ (1-\alpha) A_tK_t^{\alpha}L_t^{-\alpha}=w_t\\
\end{align}
$$
$L_t=1$
$$
\begin{align}
r_t &= \alpha A_tK_t^{\alpha-1}\\
w_t &= (1-\alpha) A_tK_t^{\alpha}
\end{align}
$$







$$
\begin{align}
&K_{t+1}-K_t=Y_t-C_t-\delta K_t=A_tK_t^\alpha -C_t-\delta K_t\\
&\Leftrightarrow~ K_{t+1}=A_tK_t^\alpha+(1-\delta) K_t -C_t
\end{align}
$$



$$
r_tK_t+w_t=\alpha A_tK_t^{\alpha-1} \times K_t +(1-\alpha) A_tK_t^{\alpha}=A_tK_t^\alpha=Y_t
$$


定常状態
$$
1=\beta(\alpha A_{t+1}K_{t+1}^{\alpha-1}+1-\delta)
$$

$$
K_t=\left( \frac{\beta^{-1}-1+\delta}{\alpha A_t} \right)^{\frac{1}{\alpha-1}}
$$

$$
K=A_tK^\alpha+(1-\delta) K -C_t ~\Rightarrow~ C_t=A_tK^\alpha-\delta K
$$

$$
K^*=\left( \frac{\beta^{-1}-1+\delta}{\alpha A_t} \right)^{\frac{1}{\alpha-1}}
$$

$$
C^*=A_t(K^*)^\alpha-\delta K^*
$$




$$
\begin{align}
C_{t+1} &= \beta(\alpha A_tK_t^{\alpha-1}+1-\delta)C_t \\
K_{t+1} &= A_tK_t^\alpha -C_t+(1-\delta) K_t
\end{align}
$$


